HybridVerifVecs/nd_funs/cat2ndfun_examples.thy
@@ -5,55 +5,14 @@ begin
 
 subsection\<open> Examples \<close>
 
+text\<open> Preliminary preparation for the examples.\<close>
+
 no_notation Archimedean_Field.ceiling ("\<lceil>_\<rceil>")
         and Archimedean_Field.floor_ceiling_class.floor ("\<lfloor>_\<rfloor>")
 
-lemma picard_lindeloef_linear_system:
-  fixes A::"real^'n^'n"
-  defines "L \<equiv> (real CARD('n))\<^sup>2 * (\<parallel>A\<parallel>\<^sub>m\<^sub>a\<^sub>x)"
-  shows "picard_lindeloef (\<lambda> t s. A *v s) UNIV UNIV 0"
-  apply(unfold_locales, simp_all add: local_lipschitz_def lipschitz_on_def, clarsimp)
-  apply(rule_tac x=1 in exI, clarsimp, rule_tac x="L" in exI, safe)
-  using max_norm_ge_0[of A] unfolding assms by force (rule matrix_lipschitz_constant)
+\<comment> \<open>Finite set of program variables.\<close>
 
-lemma picard_lindeloef_sq_mtx:
-  fixes A::"('n::finite) sqrd_matrix"
-  defines "L \<equiv> (real CARD('n))\<^sup>2 * (\<parallel>to_vec A\<parallel>\<^sub>m\<^sub>a\<^sub>x)"
-  shows "picard_lindeloef (\<lambda> t s. A *\<^sub>V s) UNIV UNIV 0"
-  apply(unfold_locales, simp_all add: local_lipschitz_def lipschitz_on_def, clarsimp)
-  apply(rule_tac x=1 in exI, clarsimp, rule_tac x="L" in exI, safe)
-  using max_norm_ge_0[of "to_vec A"] unfolding assms apply force
-  by transfer (rule matrix_lipschitz_constant)
-
-lemma local_flow_exp:
-  fixes A::"('n::finite) sqrd_matrix"
-  shows "local_flow ((*\<^sub>V) A) UNIV UNIV (\<lambda>t s. exp (t *\<^sub>R A) *\<^sub>V s)"
-  unfolding local_flow_def local_flow_axioms_def apply safe
-  using picard_lindeloef_sq_mtx apply blast
-  using exp_has_vderiv_on_linear[of 0] apply force
-  by(auto simp: sq_mtx_one_vec)
-
-text\<open> The examples in this subsection show different approaches for the verification of hybrid 
-systems. however, the general approach can be outlined as follows: First, we select a finite type to
-model program variables @{typ 'n}. We use this to define a vector field @{term f} of type
- @{typ "'a^'n \<Rightarrow> 'a^'n"} to model the dynamics of our system. Then we show a partial correctness 
-specification involving the evolution command @{term "(x\<acute>=f & S)"} either by finding a flow for 
-the vector field or through differential invariants.\<close>
-
-
-subsubsection\<open> Single constantly accelerated evolution \<close>
-
-text\<open> The main characteristics distinguishing this example from the rest are:
-\begin{enumerate}
-\item We define the finite type of program variables with 2 Isabelle strings which make the final
-verification easier to parse.
-\item We define the vector field (named @{term K}) to model a constantly accelerated object.
-\item We define a local flow (@{term \<phi>\<^sub>K}) and use it to compute the wlp for this vector field.
-\item The verification is only done on a single evolution command (not operated with any other 
-hybrid program).
-\end{enumerate} \<close>
-
-typedef program_vars ="{''x'',''v''}"
+typedef program_vars = "{''x'',''y''}"
   morphisms to_str to_var
   apply(rule_tac x="''x''" in exI)
   by simp
@@ -64,219 +23,122 @@ lemma number_of_program_vars: "CARD(program_vars) = 2"
   using type_definition.card type_definition_program_vars by fastforce
 
 instance program_vars::finite
-  apply(standard, subst bij_betw_finite[of to_str UNIV "{''x'',''v''}"])
+  apply(standard, subst bij_betw_finite[of to_str UNIV "{''x'',''y''}"])
    apply(rule bij_betwI')
      apply (simp add: to_str_inject)
   using to_str apply blast
    apply (metis to_var_inverse UNIV_I)
   by simp
 
-lemma program_vars_univD: "(UNIV::program_vars set) = {\<restriction>\<^sub>V ''x'', \<restriction>\<^sub>V ''v''}"
+lemma program_vars_univ_eq: "(UNIV::program_vars set) = {\<restriction>\<^sub>V''x'', \<restriction>\<^sub>V''y''}"
   apply auto by (metis to_str to_str_inverse insertE singletonD) 
 
-lemma program_vars_exhaust: "x = \<restriction>\<^sub>V ''x'' \<or> x = \<restriction>\<^sub>V ''v''"
-  using program_vars_univD by auto
+lemma program_vars_exhaust: "x = \<restriction>\<^sub>V''x'' \<or> x = \<restriction>\<^sub>V''y''"
+  using program_vars_univ_eq by auto
 
-abbreviation "constant_acceleration_kinematics g s \<equiv> 
-  (\<chi> i. if i=(\<restriction>\<^sub>V ''x'') then s $ (\<restriction>\<^sub>V ''v'') else g)"
+\<comment> \<open>Alternative to the finite set of program variables.\<close>
 
-notation constant_acceleration_kinematics ("K")
-
-lemma cnst_acc_continuous:
-  fixes X::"(real^program_vars) set"
-  shows "continuous_on X (K g)"
-  apply(rule continuous_on_vec_lambda)
-  unfolding continuous_on_def apply clarsimp
-  by(intro tendsto_intros)
-
-lemma picard_lindeloef_cnst_acc:
-  fixes g::real
-  shows "picard_lindeloef (\<lambda>t. K g) UNIV UNIV 0"
-  apply(unfold_locales, simp_all add: local_lipschitz_def lipschitz_on_def, clarsimp)
-  apply(rule_tac x="1/2" in exI, clarsimp, rule_tac x=1 in exI)
-  by(simp add: dist_norm norm_vec_def L2_set_def program_vars_univD to_var_inject)
-
-abbreviation "constant_acceleration_kinematics_flow g t s \<equiv> 
-  (\<chi> i. if i=(\<restriction>\<^sub>V ''x'') then g \<cdot> t ^ 2/2 + s $ (\<restriction>\<^sub>V ''v'') \<cdot> t + s $ (\<restriction>\<^sub>V ''x'') 
-        else g \<cdot> t + s $ (\<restriction>\<^sub>V ''v''))"
-
-notation constant_acceleration_kinematics_flow ("\<phi>\<^sub>K")
-
-lemma local_flow_cnst_acc: "local_flow (K g) UNIV UNIV (\<phi>\<^sub>K g)"
-  unfolding local_flow_def local_flow_axioms_def apply safe
-  using picard_lindeloef_cnst_acc apply blast
-   apply(rule has_vderiv_on_vec_lambda, clarify)
-   apply(case_tac "i = \<restriction>\<^sub>V ''x''")
-  using program_vars_exhaust by(auto intro!: poly_derivatives simp: to_var_inject vec_eq_iff)
-
-lemma single_evolution_ball:
-  fixes h::real assumes "g < 0" and "h \<ge> 0"
-  shows "\<lceil>\<lambda>s. s $ (\<restriction>\<^sub>V ''x'') = h \<and> s $ (\<restriction>\<^sub>V ''v'') = 0\<rceil> 
-  \<le> wp (x\<acute>=K g & (\<lambda> s. s $ (\<restriction>\<^sub>V ''x'') \<ge> 0))
-  \<lceil>\<lambda>s. 0 \<le> s $ (\<restriction>\<^sub>V ''x'') \<and> s $ (\<restriction>\<^sub>V ''x'') \<le> h\<rceil>"
-  apply(subst local_flow.wp_g_orbit[OF local_flow_cnst_acc], simp_all)
-  using assms by(auto simp: mult_nonneg_nonpos2)
-
-no_notation to_var ("\<restriction>\<^sub>V")
-
-no_notation constant_acceleration_kinematics ("K")
-
-no_notation constant_acceleration_kinematics_flow ("\<phi>\<^sub>K")
-
-
-subsubsection \<open>Single evolution revisited.\<close>
-
-text\<open> We list again the characteristics that distinguish this example:
-\begin{enumerate}
-\item We employ an existing finite type of size $3$ to model program variables.
-\item We define a $3\times 3$ matrix (named @{term K}) to denote the linear operator that models 
-the constantly accelerated motion.
-\item We define a local flow (@{term \<phi>\<^sub>K}) and use it to compute the wlp for this linear operator.
-\item The verification is done equivalently to the above example.
-\end{enumerate} \<close>
-
-term "x::2" \<comment> \<open>It turns out that there is already a 2-element type:\<close>
-
-lemma "CARD(program_vars) = CARD(2)"
+lemma "CARD(2) = CARD(program_vars)"
   unfolding number_of_program_vars by simp
 
-text \<open>In fact, for each natural number $n$ there is already a corresponding $n$-element type in 
-Isabelle. however, there are still lemmas to prove about them in order to do verification of hybrid
-systems in $n$-dimensional Euclidean spaces.\<close>
+lemma [simp]: "i \<noteq> (0::2) \<longrightarrow> i = 1" 
+  using exhaust_2 by fastforce
 
-lemma exhaust_5: \<comment> \<open>The analogs for $1,2$ and $3$ have already been proven in Analysis.\<close>
-  fixes x::5 
-  shows "x=1 \<or> x=2 \<or> x=3 \<or> x=4 \<or> x=5"
-proof (induct x)
-  case (of_int z)
-  then have "0 \<le> z" and "z < 5" by simp_all
-  then have "z = 0 \<or> z = 1 \<or> z = 2 \<or> z = 3 \<or> z = 4" by arith
-  then show ?case by auto
-qed
+lemma two_eq_zero: "(2::2) = 0" 
+  by simp
+
+lemma UNIV_2: "(UNIV::2 set) = {0, 1}"
+  apply safe using exhaust_2 two_eq_zero by auto
 
 lemma UNIV_3: "(UNIV::3 set) = {0, 1, 2}"
-  apply safe using exhaust_3 three_eq_zero by(blast, auto)
+  apply safe using exhaust_3 three_eq_zero by auto
 
 lemma sum_axis_UNIV_3[simp]: "(\<Sum>j\<in>(UNIV::3 set). axis i 1 $ j \<cdot> f j) = (f::3 \<Rightarrow> real) i"
   unfolding axis_def UNIV_3 apply simp
   using exhaust_3 by force
 
-text\<open> We can rewrite the original constant acceleration kinematics as a linear operator applied to 
-a 3-dimensional vector. For that we take advantage of the following fact: \<close>
 
-lemma "\<e> 1 = (\<chi> j::3. if j= 0 then 0 else if j = 1 then 1 else 0)"
-  unfolding axis_def by(rule Cart_lambda_cong, simp)
+subsubsection\<open>Circular Motion\<close>
 
-abbreviation "constant_acceleration_kinematics_matrix \<equiv> 
-  (\<chi> i::3. if i=0 then \<e> 1 else if i=1 then \<e> 2 else (0::real^3))"
+\<comment> \<open>Verified with differential invariants. \<close>
 
-abbreviation "constant_acceleration_kinematics_matrix_flow t s \<equiv> 
-  (\<chi> i::3. if i=0 then s $ 2 \<cdot> t ^ 2/2 + s $ 1 \<cdot> t + s $ 0
-   else if i=1 then s $ 2 \<cdot> t + s $ 1 else s $ 2)"
+abbreviation circular_motion_kinematics :: "real^program_vars \<Rightarrow> real^program_vars" 
+  where "circular_motion_kinematics s \<equiv> (\<chi> i. if i=(\<restriction>\<^sub>V''x'') then s$(\<restriction>\<^sub>V''y'') else -s$(\<restriction>\<^sub>V''x''))"
 
-notation constant_acceleration_kinematics_matrix ("A")
+notation circular_motion_kinematics ("C")
 
-notation constant_acceleration_kinematics_matrix_flow ("\<phi>\<^sub>A")
-
-text\<open> With these 2 definitions and the proof that linear systems of ODEs are Picard-Lindeloef, we 
-can show that they form a pair of vector-field and its flow. \<close>
-
-lemma entries_cnst_acc_matrix: "entries A = {0, 1}"
-  apply (simp_all add: axis_def, safe)
-  by(rule_tac x="1" in exI, simp)+
-
-lemma local_flow_cnst_acc_matrix: "local_flow ((*v) A) UNIV UNIV \<phi>\<^sub>A"
-  unfolding local_flow_def local_flow_axioms_def apply safe
-     apply(rule picard_lindeloef_linear_system[where A=A], simp_all add: vec_eq_iff)
-   apply(rule has_vderiv_on_vec_lambda)
-   apply(auto intro!: poly_derivatives simp: matrix_vector_mult_def vec_eq_iff)
-  using exhaust_3 by force
-
-text\<open> Finally, we compute the wlp and use it to verify the single-evolution ball again.\<close>
-
-lemma single_evolution_ball_K: 
-  "\<lceil>\<lambda>s. 0 \<le> s $ 0 \<and> s $ 0 = h \<and> s $ 1 = 0 \<and> 0 > s $ 2\<rceil> 
-  \<le> wp (x\<acute>=(*v) A & (\<lambda> s. s $ 0 \<ge> 0)) 
-  \<lceil>\<lambda>s. 0 \<le> s $ 0 \<and> s $ 0 \<le> h\<rceil>"
-  apply(subst local_flow.wp_g_orbit[of "(*v) A"])
-  using local_flow_cnst_acc_matrix apply force
-  by(auto simp: mult_nonneg_nonpos2)
-
-
-subsubsection\<open> Circular Motion \<close>
-
-text\<open> The characteristics that distinguish this example are:
-\begin{enumerate}
-\item We employ an existing finite type of size $2$ to model program variables.
-\item We define a $2\times 2$ matrix (named @{term C}) to denote the linear operator that models 
-circular motion.
-\item We show that the circle equation is a differential invariant for the linear operator.
-\item We prove the partial correctness specification corresponding to the previous point.
-\item For completeness, we define a local flow (@{term \<phi>\<^sub>C}) and use it to compute the wlp for the 
-linear operator and the specification is proven again with this flow.
-\end{enumerate} \<close>
-
-lemma two_eq_zero: "(2::2) = 0" 
-  by simp
-
-lemma [simp]: "i \<noteq> (0::2) \<longrightarrow> i = 1" 
-  using exhaust_2 by fastforce
-
-lemma UNIV_2: "(UNIV::2 set) = {0, 1}"
-  apply safe using exhaust_2 two_eq_zero by auto
-
-abbreviation circular_motion_matrix :: "real^2^2" 
-  where "circular_motion_matrix \<equiv> (\<chi> i. if i=0 then - \<e> 1 else \<e> 0)"
-
-notation circular_motion_matrix ("C")
-
-lemma circle_invariant: 
-  "diff_invariant (\<lambda>s. r\<^sup>2 = (s $ 0)\<^sup>2 + (s $ 1)\<^sup>2) ((*v) C) UNIV UNIV 0 G"
+lemma circular_motion_invariant: 
+  "diff_invariant (\<lambda>s. (r::real)\<^sup>2 = (s$(\<restriction>\<^sub>V''x''))\<^sup>2 + (s$(\<restriction>\<^sub>V''y''))\<^sup>2) C UNIV UNIV 0 G"
   apply(rule_tac diff_invariant_rules, clarsimp, simp, clarsimp)
-  apply(frule_tac i="0" in has_vderiv_on_vec_nth, drule_tac i="1" in has_vderiv_on_vec_nth)
-  apply(rule_tac S="UNIV" in has_vderiv_on_subset)
-  by(auto intro!: poly_derivatives simp: matrix_vector_mult_def)
+  apply(frule_tac i="\<restriction>\<^sub>V''x''" in has_vderiv_on_vec_nth, drule_tac i="\<restriction>\<^sub>V''y''" in has_vderiv_on_vec_nth)
+  by(auto intro!: poly_derivatives simp: to_var_inject)
 
 lemma circular_motion_invariants:
-  "\<lceil>\<lambda>s. r\<^sup>2 = (s $ 0)\<^sup>2 + (s $ 1)\<^sup>2\<rceil> \<le> wp (x\<acute>=(*v) C & G) \<lceil>\<lambda>s. r\<^sup>2 = (s $ 0)\<^sup>2 + (s $ 1)\<^sup>2\<rceil>"
-  unfolding wp_diff_inv using circle_invariant by auto
+  "\<lceil>\<lambda>s. r\<^sup>2 = (s$\<restriction>\<^sub>V''x'')\<^sup>2 + (s$\<restriction>\<^sub>V''y'')\<^sup>2\<rceil> \<le> wp (x\<acute>= C & G) \<lceil>\<lambda>s. r\<^sup>2 = (s$\<restriction>\<^sub>V''x'')\<^sup>2 + (s$\<restriction>\<^sub>V''y'')\<^sup>2\<rceil>"
+  unfolding wp_diff_inv using circular_motion_invariant by auto
 
-\<comment> \<open>Proof of the same specification by providing solutions:\<close>
+\<comment> \<open>Verified with the flow. \<close>
 
-lemma entries_circ_matrix: "entries C = {0, - 1, 1}"
-  apply (simp_all add: axis_def, safe)
-  subgoal by(rule_tac x="0" in exI, simp)+
-  subgoal by(rule_tac x="0" in exI, simp)+
-  by(rule_tac x="1" in exI, simp)+
+abbreviation "circular_motion_flow t s \<equiv> 
+  (\<chi> i. if i=\<restriction>\<^sub>V''x'' then s$(\<restriction>\<^sub>V''x'') \<cdot> cos t + s$(\<restriction>\<^sub>V''y'') \<cdot> sin t
+  else - s$(\<restriction>\<^sub>V''x'') \<cdot> sin t + s$(\<restriction>\<^sub>V''y'') \<cdot> cos t)"
 
-abbreviation "circular_motion_matrix_flow t s \<equiv> 
-  (\<chi> i. if i= (0::2) then s$0 \<cdot> cos t - s$1 \<cdot> sin t else s$0 \<cdot> sin t + s$1 \<cdot> cos t)"
+notation circular_motion_flow ("\<phi>\<^sub>C")
 
-notation circular_motion_matrix_flow ("\<phi>\<^sub>C")
+lemma picard_lindeloef_circ_motion: "picard_lindeloef (\<lambda>t. C) UNIV UNIV 0"
+  apply(unfold_locales, simp_all add: local_lipschitz_def lipschitz_on_def, clarsimp)
+  apply(rule_tac x="1" in exI, clarsimp, rule_tac x=1 in exI)
+  by(simp add: dist_norm norm_vec_def L2_set_def program_vars_univ_eq to_var_inject power2_commute)
 
-lemma local_flow_circ_matrix: "local_flow ((*v) C) UNIV UNIV \<phi>\<^sub>C"
+lemma local_flow_circ_motion: "local_flow C UNIV UNIV \<phi>\<^sub>C"
   unfolding local_flow_def local_flow_axioms_def apply safe
-  apply(rule picard_lindeloef_linear_system[where A=C], simp_all add: vec_eq_iff)
-   apply(rule has_vderiv_on_vec_lambda)
-  apply(force intro!: poly_derivatives simp: matrix_vector_mult_def)
-  using exhaust_2 two_eq_zero by(force simp: vec_eq_iff)
+  apply(rule picard_lindeloef_circ_motion, simp_all add: vec_eq_iff)
+   apply(rule has_vderiv_on_vec_lambda, clarify)
+   apply(case_tac "i = \<restriction>\<^sub>V''x''", simp)
+    apply(force intro!: poly_derivatives derivative_intros simp: to_var_inject)
+  apply(force intro!: poly_derivatives derivative_intros simp: to_var_inject)
+  using program_vars_exhaust by force
 
 lemma circular_motion:
-  "\<lceil>\<lambda>s. r\<^sup>2 = (s $ 0)\<^sup>2 + (s $ 1)\<^sup>2\<rceil> \<le> wp (x\<acute>=(*v) C & G) \<lceil>\<lambda>s. r\<^sup>2 = (s $ 0)\<^sup>2 + (s $ 1)\<^sup>2\<rceil>"
-  by(subst local_flow.wp_g_orbit[OF local_flow_circ_matrix]) auto
+  "\<lceil>\<lambda>s. r\<^sup>2 = (s$\<restriction>\<^sub>V''x'')\<^sup>2 + (s$\<restriction>\<^sub>V''y'')\<^sup>2\<rceil> \<le> wp (x\<acute>= C & G) \<lceil>\<lambda>s. r\<^sup>2 = (s$\<restriction>\<^sub>V''x'')\<^sup>2 + (s$\<restriction>\<^sub>V''y'')\<^sup>2\<rceil>"
+  by (subst local_flow.wp_g_orbit[OF local_flow_circ_motion]) (auto simp: to_var_inject)
 
-no_notation circular_motion_matrix ("C")
+no_notation circular_motion_kinematics ("C")
 
-no_notation circular_motion_matrix_flow ("\<phi>\<^sub>C")
+no_notation circular_motion_flow ("\<phi>\<^sub>C")
+
+\<comment> \<open>Verified as a linear system (using uniqueness). \<close>
+
+abbreviation circular_motion_sq_mtx :: "2 sq_mtx" 
+  where "circular_motion_sq_mtx \<equiv> sq_mtx_chi (\<chi> i. if i=0 then - \<e> 1 else \<e> 0)"
+
+abbreviation circular_motion_mtx_flow :: "real \<Rightarrow> real^2 \<Rightarrow> real^2" 
+  where "circular_motion_mtx_flow t s \<equiv> 
+  (\<chi> i. if i=(0::2) then s$0 \<cdot> cos t - s$1 \<cdot> sin t else s$0 \<cdot> sin t + s$1 \<cdot> cos t)"
+
+notation circular_motion_sq_mtx ("C")
+
+notation circular_motion_mtx_flow ("\<phi>\<^sub>C")
+
+lemma circular_motion_mtx_exp_eq: "exp (t *\<^sub>R C) *\<^sub>V s = \<phi>\<^sub>C t s"
+  apply(rule local_flow.eq_solution[OF local_flow_exp, symmetric])
+    apply(rule ivp_solsI, rule has_vderiv_on_vec_lambda, clarsimp)
+  unfolding sq_mtx_vec_prod_def matrix_vector_mult_def apply simp
+      apply(force intro!: poly_derivatives simp: matrix_vector_mult_def)
+  using exhaust_2 two_eq_zero by (force simp: vec_eq_iff, auto)
+
+lemma circular_motion_sq_mtx:
+  "\<lceil>\<lambda>s. r\<^sup>2 = (s$0)\<^sup>2 + (s$1)\<^sup>2\<rceil> \<le> wp (x\<acute>= ((*\<^sub>V) C) & G) \<lceil>\<lambda>s. r\<^sup>2 = (s$0)\<^sup>2 + (s$1)\<^sup>2\<rceil>"
+  unfolding local_flow.wp_g_orbit[OF local_flow_exp] circular_motion_mtx_exp_eq by auto
+
+no_notation circular_motion_sq_mtx ("C")
+
+no_notation circular_motion_mtx_flow ("\<phi>\<^sub>C")
 
 
-subsubsection\<open> Bouncing Ball with solution \<close>
+subsubsection\<open> Bouncing Ball \<close>
 
-text\<open> We revisit the previous dynamics for a constantly accelerated object modelled with the matrix
-@{term K}. We compose the corresponding evolution command with an if-statement, and iterate this 
-hybrid program to model a (completely elastic) ``bouncing ball''. Using the previously defined flow
-for this dynamics, proving a specification for this hybrid program is merely an exercise of real 
-arithmetic. \<close>
+\<comment> \<open>Verified with differential invariants. \<close>
 
 named_theorems bb_real_arith "real arithmetic properties for the bouncing ball."
 
@@ -297,11 +159,68 @@ proof-
   thus ?thesis by auto
 qed
 
+abbreviation "constant_acceleration_kinematics g s \<equiv> (\<chi> i. if i=(\<restriction>\<^sub>V''x'') then s$(\<restriction>\<^sub>V''y'') else g)"
+
+notation constant_acceleration_kinematics ("K")
+
+lemma energy_conservation_invariant: 
+  fixes g h :: real
+  defines dinv: "I \<equiv> (\<lambda>s. 2 \<cdot> g \<cdot> s$(\<restriction>\<^sub>V''x'') - 2 \<cdot> g \<cdot> h - (s$(\<restriction>\<^sub>V''y'') \<cdot> s$(\<restriction>\<^sub>V''y'')) = 0)"
+  shows "diff_invariant I (K g) UNIV UNIV 0 G"
+  unfolding dinv apply(rule diff_invariant_rules, simp, simp, clarify)
+  apply(frule_tac i="\<restriction>\<^sub>V''y''" in has_vderiv_on_vec_nth)
+  apply(drule_tac i="\<restriction>\<^sub>V''x''" in has_vderiv_on_vec_nth)
+  by(auto intro!: poly_derivatives simp: to_var_inject)
+
+lemma bouncing_ball_invariants:
+  fixes h::real 
+  assumes "g < 0" and "h \<ge> 0"
+  defines diff_inv: "I \<equiv> (\<lambda>s. 2 \<cdot> g \<cdot> s$(\<restriction>\<^sub>V''x'') - 2 \<cdot> g \<cdot> h - (s$(\<restriction>\<^sub>V''y'') \<cdot> s$(\<restriction>\<^sub>V''y'')) = 0)"
+  shows "\<lceil>\<lambda>s. s$(\<restriction>\<^sub>V''x'') = h \<and> s$(\<restriction>\<^sub>V''y'') = 0\<rceil> \<le> 
+  wp (((x\<acute>=K g & (\<lambda> s. s$(\<restriction>\<^sub>V''x'') \<ge> 0)) \<cdot>
+  (IF (\<lambda> s. s$(\<restriction>\<^sub>V''x'') = 0) THEN ((\<restriction>\<^sub>V''y'') ::= (\<lambda>s. - s$(\<restriction>\<^sub>V''y''))) ELSE \<eta>\<^sup>\<bullet> FI))\<^sup>\<star>)
+  \<lceil>\<lambda>s. 0 \<le> s$(\<restriction>\<^sub>V''x'') \<and> s$(\<restriction>\<^sub>V''x'') \<le> h\<rceil>"
+  apply(subst star_nd_fun.abs_eq)
+  apply(rule_tac I="\<lceil>\<lambda>s. 0 \<le> s$(\<restriction>\<^sub>V''x'') \<and> I s\<rceil>" in wp_starI)
+  using \<open>h \<ge> 0\<close> apply(simp add: diff_inv, simp only: fbox_mult)
+   apply(subst p2ndf_ndf2p_wp[symmetric, of "(IF _ THEN _ ELSE \<eta>\<^sup>\<bullet> FI)"])
+   apply(rule order.trans[where b="wp (x\<acute>=K g & (\<lambda>s. s$(\<restriction>\<^sub>V''x'')\<ge>0)) \<lceil>\<lambda>s. 0\<le>s$(\<restriction>\<^sub>V''x'') \<and> I s\<rceil>"])
+    apply(simp only: wp_g_evolution_guard)
+    apply(rule order.trans[where b="\<lceil>I\<rceil>"], simp)
+    apply(simp add: wp_diff_inv, unfold diff_inv)
+  using energy_conservation_invariant apply force
+   apply(rule fbox_iso)
+   apply(simp add: plus_nd_fun_def f2r_def times_nd_fun_def kcomp_def)
+  using assms by (auto simp: bb_real_arith le_fun_def)
+
+
+\<comment> \<open>Verified with the flow. \<close>
+
+lemma picard_lindeloef_cnst_acc:
+  fixes g::real
+  shows "picard_lindeloef (\<lambda>t. K g) UNIV UNIV 0"
+  apply(unfold_locales)
+  apply(unfold_locales, simp_all add: local_lipschitz_def lipschitz_on_def, clarsimp)
+  apply(rule_tac x="1/2" in exI, clarsimp, rule_tac x=1 in exI)
+  by(simp add: dist_norm norm_vec_def L2_set_def program_vars_univ_eq to_var_inject)
+
+abbreviation "constant_acceleration_kinematics_flow g t s \<equiv> 
+  (\<chi> i. if i=(\<restriction>\<^sub>V ''x'') then g \<cdot> t ^ 2/2 + s $ (\<restriction>\<^sub>V ''y'') \<cdot> t + s $ (\<restriction>\<^sub>V ''x'') 
+        else g \<cdot> t + s $ (\<restriction>\<^sub>V ''y''))"
+
+notation constant_acceleration_kinematics_flow ("\<phi>\<^sub>K")
+
+lemma local_flow_cnst_acc: "local_flow (K g) UNIV UNIV (\<phi>\<^sub>K g)"
+  unfolding local_flow_def local_flow_axioms_def apply safe
+  using picard_lindeloef_cnst_acc apply blast
+   apply(rule has_vderiv_on_vec_lambda, clarify)
+   apply(case_tac "i = \<restriction>\<^sub>V ''x''")
+  using program_vars_exhaust by(auto intro!: poly_derivatives simp: to_var_inject vec_eq_iff)
+
 lemma [bb_real_arith]:
   assumes invar: "2 \<cdot> g \<cdot> x = 2 \<cdot> g \<cdot> h + v \<cdot> v"
     and pos: "g \<cdot> \<tau>\<^sup>2 / 2 + v \<cdot> \<tau> + (x::real) = 0"
-  shows "2 \<cdot> g \<cdot> h + (- (g \<cdot> \<tau>) - v) \<cdot> (- (g \<cdot> \<tau>) - v) = 0"
-    and "2 \<cdot> g \<cdot> h + (g \<cdot> \<tau> \<cdot> (g \<cdot> \<tau> + v) + v \<cdot> (g \<cdot> \<tau> + v)) = 0"
+  shows "2 \<cdot> g \<cdot> h + (g \<cdot> \<tau> \<cdot> (g \<cdot> \<tau> + v) + v \<cdot> (g \<cdot> \<tau> + v)) = 0"
 proof-
   from pos have "g \<cdot> \<tau>\<^sup>2  + 2 \<cdot> v \<cdot> \<tau> + 2 \<cdot> x = 0" by auto
   then have "g\<^sup>2  \<cdot> \<tau>\<^sup>2  + 2 \<cdot> g \<cdot> v \<cdot> \<tau> + 2 \<cdot> g \<cdot> x = 0"
@@ -316,10 +235,8 @@ proof-
     by (simp add: monoid_mult_class.power2_eq_square)
   have  "2 \<cdot> g \<cdot> h + (- ((g \<cdot> \<tau>) + v))\<^sup>2 = 0"
     using obs by (metis Groups.add_ac(2) power2_minus)
-  thus "2 \<cdot> g \<cdot> h + (- (g \<cdot> \<tau>) - v) \<cdot> (- (g \<cdot> \<tau>) - v) = 0"
-    by (simp add: monoid_mult_class.power2_eq_square)
 qed
-    
+
 lemma [bb_real_arith]:
   assumes invar: "2 \<cdot> g \<cdot> x = 2 \<cdot> g \<cdot> h + v \<cdot> v"
   shows "2 \<cdot> g \<cdot> (g \<cdot> \<tau>\<^sup>2 / 2 + v \<cdot> \<tau> + (x::real)) = 
@@ -341,139 +258,58 @@ proof-
 qed
 
 lemma bouncing_ball:
-  "\<lceil>\<lambda>s. 0 \<le> s $ 0 \<and> s $ 0 = h \<and> s $ 1 = 0 \<and> 0 > s $ 2\<rceil> \<le> 
-  wp (((x\<acute>=(*v) A & (\<lambda> s. s $ 0 \<ge> 0)) \<cdot>
-  (IF (\<lambda> s. s $ 0 = 0) THEN (1 ::= (\<lambda>s. - s $ 1)) ELSE \<eta>\<^sup>\<bullet> FI))\<^sup>\<star>)
-  \<lceil>\<lambda>s. 0 \<le> s $ 0 \<and> s $ 0 \<le> h\<rceil>"
+  fixes h::real 
+  assumes "g < 0" and "h \<ge> 0"
+  defines loop_inv: "I \<equiv> (\<lambda>s. 0 \<le> s$(\<restriction>\<^sub>V''x'') \<and>  2 \<cdot> g \<cdot> s$(\<restriction>\<^sub>V''x'') = 
+    2 \<cdot> g \<cdot> h + (s$(\<restriction>\<^sub>V''y'') \<cdot> s$(\<restriction>\<^sub>V''y'')))"
+  shows "\<lceil>\<lambda>s. s$(\<restriction>\<^sub>V''x'') = h \<and> s$(\<restriction>\<^sub>V''y'') = 0\<rceil> \<le> 
+  wp (((x\<acute>=K g & (\<lambda> s. s$(\<restriction>\<^sub>V''x'') \<ge> 0)) \<cdot>
+  (IF (\<lambda> s. s$(\<restriction>\<^sub>V''x'') = 0) THEN ((\<restriction>\<^sub>V''y'') ::= (\<lambda>s. - s$(\<restriction>\<^sub>V''y''))) ELSE \<eta>\<^sup>\<bullet> FI))\<^sup>\<star>)
+  \<lceil>\<lambda>s. 0 \<le> s$(\<restriction>\<^sub>V''x'') \<and> s$(\<restriction>\<^sub>V''x'') \<le> h\<rceil>"
   apply(subst star_nd_fun.abs_eq)
-  apply(rule_tac I="\<lceil>\<lambda>s. 0 \<le> s $ 0 \<and> 0 > s $ 2 \<and> 
-  2 \<cdot> s $ 2 \<cdot> s $ 0 = 2 \<cdot> s $ 2 \<cdot> h + (s $ 1 \<cdot> s $ 1)\<rceil>" in wp_starI)
-    apply(simp, simp only: fbox_mult)
-   apply(subst p2ndf_ndf2p_wp[symmetric, of "(IF (\<lambda>s. s $ 0 = 0) THEN (1 ::= (\<lambda>s. - s $ 1)) ELSE \<eta>\<^sup>\<bullet> FI)"])
-   apply(subst local_flow.wp_g_orbit[OF local_flow_cnst_acc_matrix], simp, subst ndf2p_wpD)
-  unfolding cond_def apply clarsimp
-  by (transfer, simp add: kcomp_def) (auto simp: bb_real_arith)
+  apply(rule_tac I="\<lceil>I\<rceil>" in wp_starI)
+   unfolding loop_inv using \<open>h \<ge> 0\<close> apply(simp, simp only: fbox_mult)
+   apply(subst p2ndf_ndf2p_wp[symmetric, of "(IF _ THEN _ ELSE \<eta>\<^sup>\<bullet> FI)"])
+    apply(subst local_flow.wp_g_orbit[OF local_flow_cnst_acc])
+   apply(subst ndf2p_wpD)
+  unfolding cond_def apply(simp add: plus_nd_fun_def f2r_def times_nd_fun_def kcomp_def)
+  using assms by (auto simp: bb_real_arith le_fun_def to_var_inject)
 
+no_notation constant_acceleration_kinematics ("K")
 
-subsubsection\<open> Bouncing Ball with invariants \<close>
+no_notation constant_acceleration_kinematics_flow ("\<phi>\<^sub>K")
 
-text\<open> We prove again the bouncing ball but this time with differential invariants. \<close>
+no_notation to_var ("\<restriction>\<^sub>V")
 
-lemma gravity_invariant: "diff_invariant (\<lambda>s. s $ 2 < 0) ((*v) A) UNIV UNIV 0 G"
-  apply(rule_tac \<mu>'="\<lambda>s. 0" and \<nu>'="\<lambda>s. 0" in diff_invariant_rules(3), clarsimp, simp, clarsimp)
-  apply(drule_tac i="2" in has_vderiv_on_vec_nth)
-  apply(rule_tac S="UNIV" in has_vderiv_on_subset)
-  by(auto intro!: poly_derivatives simp: vec_eq_iff matrix_vector_mult_def)
+\<comment> \<open>Verified as a linear system (computing exponential). \<close>
 
-lemma energy_conservation_invariant: 
-  "diff_invariant (\<lambda>s. 2 \<cdot> s$2 \<cdot> s$0 - 2 \<cdot> s$2 \<cdot> h - s$1 \<cdot> s $ 1 = 0) ((*v) A) UNIV UNIV 0 G"
-  apply(rule diff_invariant_rules, simp, simp, clarify)
-  apply(frule_tac i="2" in has_vderiv_on_vec_nth)
-  apply(frule_tac i="1" in has_vderiv_on_vec_nth)
-  apply(drule_tac i="0" in has_vderiv_on_vec_nth)
-  apply(rule_tac S="UNIV" in has_vderiv_on_subset)
-  by(auto intro!: poly_derivatives simp: vec_eq_iff matrix_vector_mult_def)
-
-lemma bouncing_ball_invariants: 
-  fixes h::real
-  defines dinv: "I \<equiv> \<lambda>s::real^3. s $ 2 < 0 \<and> 2 \<cdot> s$2 \<cdot> s$0 - 2 \<cdot> s$2 \<cdot> h - (s$1 \<cdot> s$1) = 0"
-  shows "\<lceil>\<lambda>s. 0 \<le> s $ 0 \<and> s $ 0 = h \<and> s $ 1 = 0 \<and> 0 > s $ 2\<rceil> \<le> 
-  wp (((x\<acute>=(*v) A & (\<lambda> s. s $ 0 \<ge> 0)) \<cdot>
-  (IF (\<lambda> s. s $ 0 = 0) THEN (1 ::= (\<lambda>s. - s $ 1)) ELSE \<eta>\<^sup>\<bullet> FI))\<^sup>\<star>)
-  \<lceil>\<lambda>s. 0 \<le> s $ 0 \<and> s $ 0 \<le> h\<rceil>"
-  apply(subst star_nd_fun.abs_eq)
-  apply(rule_tac I="\<lceil>\<lambda>s. 0 \<le> s$0 \<and> I s\<rceil>" in wp_starI)
-    apply(simp add: dinv, simp only: fbox_mult)
-   apply(subst p2ndf_ndf2p_wp[symmetric, of "(IF (\<lambda>s. s $ 0 = 0) THEN (1 ::= (\<lambda>s. - s $ 1)) ELSE \<eta>\<^sup>\<bullet> FI)"])
-   apply(rule order.trans[where b="wp (x\<acute>=(*v) A & (\<lambda> s. s $ 0 \<ge> 0)) \<lceil>\<lambda>s. 0 \<le> s$0 \<and> I s\<rceil>"])
-    apply(simp only: wp_g_evolution_guard)
-    apply(rule order.trans[where b="\<lceil>I\<rceil>"], simp)
-    apply(subst wp_diff_inv, unfold dinv)
-    apply(rule diff_invariant_rules)
-  using gravity_invariant apply force
-  using energy_conservation_invariant apply force
-   apply(rule fbox_iso)
-   apply(simp add: plus_nd_fun_def f2r_def times_nd_fun_def kcomp_def )
-  by(auto simp: bb_real_arith le_fun_def)
-
-no_notation constant_acceleration_kinematics_matrix ("A")
-
-no_notation constant_acceleration_kinematics_matrix_flow ("\<phi>\<^sub>A")
-
-
-subsubsection\<open> Bouncing Ball with exponential solution \<close>
-
-text\<open> In our final example, we prove again the bouncing ball specification but this time we do it 
-with the general solution for linear systems.\<close>
-
-abbreviation "constant_acceleration_kinematics_sq_mtx \<equiv> 
-  sq_mtx_chi constant_acceleration_kinematics_matrix"
+abbreviation constant_acceleration_kinematics_sq_mtx :: "3 sq_mtx" 
+  where "constant_acceleration_kinematics_sq_mtx \<equiv> 
+    sq_mtx_chi (\<chi> i::3. if i=0 then \<e> 1 else if i=1 then \<e> 2 else 0)"
 
 notation constant_acceleration_kinematics_sq_mtx ("K")
 
-lemma max_norm_cnst_acc_sq_mtx: "\<parallel>to_vec K\<parallel>\<^sub>m\<^sub>a\<^sub>x = 1"
-proof-
-  have "{to_vec K $ i $ j |i j. i \<in> UNIV \<and> j \<in> UNIV} = {0, 1}"
-    apply (simp_all add: axis_def, safe)
-    by(rule_tac x="1" in exI, simp)+
-  thus ?thesis
-    by auto
-qed
-
-lemma const_acc_mtx_pow2: "(\<tau> *\<^sub>R K)\<^sup>2 = sq_mtx_chi (\<chi> i. if i=0 then \<tau>\<^sup>2 *\<^sub>R \<e> 2 else 0)"
-  unfolding monoid_mult_class.power2_eq_square apply(simp add: scaleR_sqrd_matrix_def)
-  unfolding times_sqrd_matrix_def apply(simp add: sq_mtx_chi_inject vec_eq_iff)
-  apply(simp add: matrix_matrix_mult_def)
-  unfolding UNIV_3 by(auto simp: axis_def)
+lemma const_acc_mtx_pow2: "K\<^sup>2 = sq_mtx_chi (\<chi> i. if i=0 then \<e> 2 else 0)"
+  unfolding power2_eq_square times_sq_mtx_def 
+  by(simp add: sq_mtx_chi_inject vec_eq_iff matrix_matrix_mult_def)
 
 lemma const_acc_mtx_powN: "n > 2 \<Longrightarrow> (\<tau> *\<^sub>R K)^n = 0"
-proof(induct n)
-  case 0
-  thus ?case by simp
-next
-  case (Suc n)
-  assume IH: "2 < n \<Longrightarrow> (\<tau> *\<^sub>R K)^n = 0" and "2 < Suc n"
-  then show ?case 
-  proof(cases "n \<le> 2")
-    case True
-    hence "n = 2"
-      using \<open>2 < Suc n\<close> le_less_Suc_eq by blast 
-    hence "(\<tau> *\<^sub>R K)^(Suc n) = (\<tau> *\<^sub>R K)^3"
-      by simp
-    also have "... = (\<tau> *\<^sub>R K) \<cdot> (\<tau> *\<^sub>R K)^2"
-      by (metis (no_types, lifting) \<open>n = 2\<close> calculation power_class.power.power_Suc)
-    also have "... = (\<tau> *\<^sub>R K) \<cdot> sq_mtx_chi (\<chi> i. if i=0 then \<tau>\<^sup>2 *\<^sub>R \<e> 2 else 0)"
-      by (subst const_acc_mtx_pow2) simp
-    also have "... = 0"
-      unfolding times_sqrd_matrix_def zero_sqrd_matrix_def
-      apply(simp add: sq_mtx_chi_inject vec_eq_iff scaleR_sqrd_matrix_def)
-      apply(simp add: matrix_matrix_mult_def)
-      unfolding UNIV_3 by(auto simp: axis_def)
-    finally show ?thesis .
-  next
-    case False
-    thus ?thesis 
-      using IH by auto
-  qed
-qed
-
-lemma suminf_eq_sum:
-  fixes f :: "nat \<Rightarrow> ('a::real_normed_vector)"
-  assumes "\<And>n. n > m \<Longrightarrow> f n = 0"
-  shows "(\<Sum>n. f n) = (\<Sum>n \<le> m. f n)"
-  using assms by (meson atMost_iff finite_atMost not_le suminf_finite)
+  apply(induct n, simp, case_tac "n \<le> 2")
+   apply(simp only: le_less_Suc_eq power_Suc, simp)
+  by(auto simp: const_acc_mtx_pow2 sq_mtx_chi_inject vec_eq_iff 
+      times_sq_mtx_def zero_sq_mtx_def matrix_matrix_mult_def)
 
 lemma exp_cnst_acc_sq_mtx: "exp (\<tau> *\<^sub>R K) = ((\<tau> *\<^sub>R K)\<^sup>2/\<^sub>R 2) + (\<tau> *\<^sub>R K) + 1"
   unfolding exp_def apply(subst suminf_eq_sum[of 2])
   using const_acc_mtx_powN by (simp_all add: numeral_2_eq_2)
- 
+
 lemma exp_cnst_acc_sq_mtx_simps:
- "exp (\<tau> *\<^sub>R K) $$ 0 $ 0 = 1" "exp (\<tau> *\<^sub>R K) $$ 0 $ 1 = \<tau>" "exp (\<tau> *\<^sub>R K) $$ 0 $ 2 = \<tau>^2/2"
- "exp (\<tau> *\<^sub>R K) $$ 1 $ 0 = 0" "exp (\<tau> *\<^sub>R K) $$ 1 $ 1 = 1" "exp (\<tau> *\<^sub>R K) $$ 1 $ 2 = \<tau>"
- "exp (\<tau> *\<^sub>R K) $$ 2 $ 0 = 0" "exp (\<tau> *\<^sub>R K) $$ 2 $ 1 = 0" "exp (\<tau> *\<^sub>R K) $$ 2 $ 2 = 1"
-  unfolding exp_cnst_acc_sq_mtx const_acc_mtx_pow2 
-  by(auto simp: plus_sqrd_matrix_def scaleR_sqrd_matrix_def one_sqrd_matrix_def mat_def 
-      scaleR_vec_def axis_def plus_vec_def)
+  "exp (\<tau> *\<^sub>R K) $$ 0 $ 0 = 1" "exp (\<tau> *\<^sub>R K) $$ 0 $ 1 = \<tau>" "exp (\<tau> *\<^sub>R K) $$ 0 $ 2 = \<tau>^2/2"
+  "exp (\<tau> *\<^sub>R K) $$ 1 $ 0 = 0" "exp (\<tau> *\<^sub>R K) $$ 1 $ 1 = 1" "exp (\<tau> *\<^sub>R K) $$ 1 $ 2 = \<tau>"
+  "exp (\<tau> *\<^sub>R K) $$ 2 $ 0 = 0" "exp (\<tau> *\<^sub>R K) $$ 2 $ 1 = 0" "exp (\<tau> *\<^sub>R K) $$ 2 $ 2 = 1"
+  unfolding exp_cnst_acc_sq_mtx scaleR_power const_acc_mtx_pow2
+  by (auto simp: plus_sq_mtx_def scaleR_sq_mtx_def one_sq_mtx_def 
+      mat_def scaleR_vec_def axis_def plus_vec_def)
 
 lemma bouncing_ball_K: 
   "\<lceil>\<lambda>s. 0 \<le> s $ 0 \<and> s $ 0 = h \<and> s $ 1 = 0 \<and> 0 > s $ 2\<rceil> \<le> 
@@ -481,18 +317,19 @@ lemma bouncing_ball_K:
   (IF (\<lambda> s. s $ 0 = 0) THEN (1 ::= (\<lambda>s. - s $ 1)) ELSE \<eta>\<^sup>\<bullet> FI))\<^sup>\<star>)
   \<lceil>\<lambda>s. 0 \<le> s $ 0 \<and> s $ 0 \<le> h\<rceil>"
     apply(subst star_nd_fun.abs_eq)
-  apply(rule_tac I="\<lceil>\<lambda>s. 0 \<le> s $ 0 \<and> 0 > s $ 2 \<and> 
-  2 \<cdot> s $ 2 \<cdot> s $ 0 = 2 \<cdot> s $ 2 \<cdot> h + (s $ 1 \<cdot> s $ 1)\<rceil>" in wp_starI)
+  apply(rule_tac I="\<lceil>\<lambda>s. 0\<le>s$0 \<and> 0 > s$2 \<and> 2 \<cdot> s$2 \<cdot> s$0 = 2 \<cdot> s$2 \<cdot> h + (s$1 \<cdot> s$1)\<rceil>" in wp_starI)
     apply(simp, simp only: fbox_mult)
-   apply(subst p2ndf_ndf2p_wp[symmetric, of "(IF (\<lambda>s. s $ 0 = 0) THEN (1 ::= (\<lambda>s. - s $ 1)) ELSE \<eta>\<^sup>\<bullet> FI)"])
-   apply(subst local_flow.wp_g_orbit[OF local_flow_exp], simp)
-  unfolding wp_nd_fun2 apply(simp add: f2r_def cond_def plus_nd_fun_def 
-      times_nd_fun_def kcomp_def sq_mtx_vec_prod_eq)
-  unfolding UNIV_3 image_le_pred apply(simp add: exp_cnst_acc_sq_mtx_simps, safe)
-  subgoal for x using bb_real_arith(3)[of "x $ 2"]
+   apply(subst p2ndf_ndf2p_wp[symmetric, of "(IF _ THEN _ ELSE \<eta>\<^sup>\<bullet> FI)"])
+   apply(subst local_flow.wp_g_orbit[OF local_flow_exp], clarsimp)
+   apply(simp add: plus_nd_fun_def times_nd_fun_def f2r_def kcomp_def)
+   apply(rule_tac x="exp (t *\<^sub>R K) *\<^sub>V s" in exI)
+ apply(simp add: sq_mtx_vec_prod_def matrix_vector_mult_def)
+  unfolding UNIV_3 apply(simp add: exp_cnst_acc_sq_mtx_simps, safe)
+  subgoal for x using bb_real_arith(2)[of "x $ 2"]
     by (simp add: add.commute mult.commute)
-  subgoal for x \<tau> using bb_real_arith(4)[where g="x $ 2" and v="x $ 1"]
+  subgoal for x \<tau> using bb_real_arith(3)[where g="x $ 2" and v="x $ 1"]
     by(simp add: add.commute mult.commute)
+  apply(simp add: field_simps power2_eq_square)
   by (force simp: bb_real_arith)
 
 no_notation constant_acceleration_kinematics_sq_mtx ("K")
